yalla/atoms.v
@@ -92,13 +92,13 @@ match n with
 end.
 
 Lemma option_nat_into_nat : embedding (option nat) nat.
-Proof. exists (nat_to_option_nat, option_nat_to_nat); intros []; reflexivity. Qed.
+Proof. exists (nat_to_option_nat, option_nat_to_nat). intros []; reflexivity. Qed.
 
 Lemma injective_option_nat_to_nat : injective option_nat_to_nat.
-Proof. apply section_injective with nat_to_option_nat; intros []; reflexivity. Qed.
+Proof. apply section_injective with nat_to_option_nat. intros []; reflexivity. Qed.
 
 Lemma nat_bijective_nat : nat_bijective nat.
-Proof. exists id; apply id_bijective. Qed.
+Proof. exists id. apply id_bijective. Qed.
 
 Definition Nat_FullAtoms := {|
   FAtom := nat_infdectype;
